Ethereum/Wheels.lean
@@ -27,8 +27,10 @@ lemma BE_le' {n : ℕ} : (BE n).size ≤ ((Nat.log2 n)/8) + 1 := by
 def BEwithSizeProof (n : ℕ) : { b : ByteArray // b.size ≤ ((Nat.log2 n)/8) + 1 } :=
   ⟨BE n, BE_le'⟩
 
-theorem ByteArray_zeroes_size : ∀ n, (ffi.ByteArray.zeroes n).size = n := by
-  intro n; simp [ffi.ByteArray.zeroes, ← ByteArray.size_data, Array.size_replicate]
+def ByteArray.zeroes (n : Nat) : ByteArray := ByteArray.mk <| Array.replicate n (0 : UInt8)
+
+theorem ByteArray_zeroes_size : ∀ n, (ByteArray.zeroes n).size = n := by
+  intro n; simp [ByteArray.zeroes, ← ByteArray.size_data, Array.size_replicate]
 
 namespace Ethereum
 
@@ -36,11 +38,11 @@ def chainId : ℕ := 1
 
 def UInt256.toByteArray (val : UInt256) : ByteArray :=
   let b := BE val.toNat
-  ffi.ByteArray.zeroes (32 - b.size) ++ b
+  ByteArray.zeroes (32 - b.size) ++ b
 
 def UInt256.toByteArrayWithSizeProof (val : UInt256) : { b : ByteArray // b.size = 32 } :=
   let b := BE val.toNat
-  let pad := ffi.ByteArray.zeroes (32 - b.size)
+  let pad := ByteArray.zeroes (32 - b.size)
   ⟨pad ++ b,
     by
       simp
@@ -82,11 +84,11 @@ lemma ofUInt256_ofNat (a : AccountAddress) :
 
 def toByteArray (a : AccountAddress) : ByteArray :=
   let b := BE a
-  ffi.ByteArray.zeroes (20 - b.size) ++ b
+  ByteArray.zeroes (20 - b.size) ++ b
 
 def toByteArrayWithSizeProof (a : AccountAddress) : { b : ByteArray // b.size = 20 }  :=
   let b := BE a
-  let pad := ffi.ByteArray.zeroes (20 - b.size)
+  let pad := ByteArray.zeroes (20 - b.size)
   ⟨pad ++ b,
     by
       simp
@@ -254,7 +256,7 @@ def ByteArray.readBytes (source : ByteArray) (start size : ℕ) : ByteArray :=
       source.copySlice start empty 0 size
     else
       ⟨⟨source.toList.drop start |>.take size⟩⟩
-  read ++ ffi.ByteArray.zeroes (size - read.size)
+  read ++ ByteArray.zeroes (size - read.size)
 
 def ByteArray.readWithoutPadding (source : ByteArray) (addr len : ℕ) : ByteArray :=
   if addr ≥ source.size then .empty else
@@ -268,7 +270,7 @@ def ByteArray.readWithPadding (source : ByteArray) (addr len : ℕ) : ByteArray 
     panic! s!"ByteArray.readWithPadding: can not handle byte arrays of length {len}"
   else
     let read := source.readWithoutPadding addr len
-    read ++ ffi.ByteArray.zeroes (len - read.size)
+    read ++ ByteArray.zeroes (len - read.size)
 
 inductive 𝕋 where
   | 𝔹 : ByteArray → 𝕋
@@ -456,14 +458,14 @@ def ByteArray.write
     if sourceAddr ≥ source.size then
       let len := min len (dest.size - destAddr)
       let destAddr := min destAddr dest.size
-      (ffi.ByteArray.zeroes len).copySlice 0 dest destAddr len
+      (ByteArray.zeroes len).copySlice 0 dest destAddr len
     else
       let practicalLen := min len (source.size - sourceAddr)
       let endPaddingAddr := min dest.size (destAddr + len)
       let sourcePaddingLength : ℕ := endPaddingAddr - (destAddr + practicalLen)
-      let sourcePadding := ffi.ByteArray.zeroes sourcePaddingLength
+      let sourcePadding := ByteArray.zeroes sourcePaddingLength
       let destPaddingLength : ℕ := destAddr - dest.size
-      let destPadding := ffi.ByteArray.zeroes destPaddingLength
+      let destPadding := ByteArray.zeroes destPaddingLength
       (source ++ sourcePadding).copySlice sourceAddr
         (dest ++ destPadding)
         destAddr
